src/1/selftest.sml
@@ -359,7 +359,7 @@ val _ = tpp "RM* p q"
 val _ = clear_overloads_on "RM*"
 
 val _ = add_rule {term_name = "=",
-                  fixity = Infix(NONASSOC, 100),
+                  fixity = Infix(NONASSOC, 450),
                   block_style = (AroundSamePrec, (PP.CONSISTENT,0)),
                   paren_style = OnlyIfNecessary,
                   pp_elements = [HardSpace 1, TOK "=", BreakSpace(1,2)]}
@@ -437,8 +437,8 @@ val _ = app tpp [
   ("!x. x /\\ y", concat ["!", bx, ". ", bx, " /\\ ", fy]),
   ("let x = p in x /\\ y",
    concat ["let ",bx, " = ", fp, " in ", bx, " /\\ ", fy]),
-  ("let f x = x /\\ p in f x /\\ y",
-   concat ["let ",bound "f", " ", bx, " = ", bx, " /\\ ", fp, " in ",
+  ("let f x = (x /\\ p) in f x /\\ y",
+   concat ["let ",bound "f", " ", bx, " = (", bx, " /\\ ", fp, ") in ",
            bound "f", " ", fx, " /\\ ", fy]),
   ("!(x:'a)::p (x:'a). q x",
    concat ["!",bx,"::",fp, " ", fx,". ",free "q"," ",bx]),
@@ -457,29 +457,29 @@ val condprinter_tests =
     [
       {input = "if oless e1 e2 /\\ oless x y /\\ foobabbbbbbb\n\
                \then p /\\ q /\\ r /\\ ppppp xxxx yyyyy\n\
-               \else if (e1 = e2) /\\ k1 <> k2\n\
-               \then T else if (e1 = e2) /\\ (k1 = k2) /\\ oless t1 t2\n\
+               \else if (e1:'a) = e2 /\\ (k1:'a) <> k2\n\
+               \then T else if e1 = e2 /\\ k1 = k2 /\\ oless t1 t2\n\
                \then T else F",
        testf = K ("Large COND 1"),
        output = "if oless e1 e2 /\\ oless x y /\\ foobabbbbbbb then\n\
                 \  p /\\ q /\\ r /\\ ppppp xxxx yyyyy\n\
-                \else if (e1 = e2) /\\ k1 <> k2 then T\n\
-                \else if (e1 = e2) /\\ (k1 = k2) /\\ oless t1 t2 then T\n\
+                \else if e1 = e2 /\\ k1 <> k2 then T\n\
+                \else if e1 = e2 /\\ k1 = k2 /\\ oless t1 t2 then T\n\
                 \else F"},
       {input = "if oless e1 e2 /\\ oless x y /\\ foobabb\n\
                \then p /\\ q /\\ r /\\ ppppp xxxx\n\
-               \else if (e1 = e2) /\\ k1 <> k2\n\
-               \then T else if (e1 = e2) /\\ (k1 = k2) /\\ oless t1 t2\n\
+               \else if e1 = e2 /\\ k1 <> k2\n\
+               \then T else if e1 = e2 /\\ k1 = k2 /\\ oless t1 t2\n\
                \then T else F",
        testf = K ("Large COND 2"),
        output = "if oless e1 e2 /\\ oless x y /\\ foobabb then\
                 \ p /\\ q /\\ r /\\ ppppp xxxx\n\
-                \else if (e1 = e2) /\\ k1 <> k2 then T\n\
-                \else if (e1 = e2) /\\ (k1 = k2) /\\ oless t1 t2 then T\n\
+                \else if e1 = e2 /\\ k1 <> k2 then T\n\
+                \else if e1 = e2 /\\ k1 = k2 /\\ oless t1 t2 then T\n\
                 \else F"},
       {input = "if really quite a long guard when looked at closely then\n\
-               \  let quite_a_long_variable_name = another_long_name \\/ x ;\n\
-               \      another_longish_name = y \\/ z\n\
+               \  let quite_a_long_variable_name = (another_long_name \\/ x);\n\
+               \      another_longish_name = (y \\/ z)\n\
                \  in\n\
                \      f x\n\
                \else\n\
@@ -487,8 +487,8 @@ val condprinter_tests =
        testf = K "Large then-branch",
        output = "if really quite a long guard when looked at closely then\n\
                 \  (let\n\
-                \     quite_a_long_variable_name = another_long_name \\/ x ;\n\
-                \     another_longish_name = y \\/ z\n\
+                \     quite_a_long_variable_name = (another_long_name \\/ x) ;\
+              \\n     another_longish_name = (y \\/ z)\n\
                 \   in\n\
                 \     f x)\n\
                 \else g y"},
